chore: move some material out of `Init.Data.String.Basic` (#10893)
This PR splits some low-hanging fruit out of `Init.Data.String.Basic`:
basic material about `String.Pos.Raw`, `String.Substrig`, and
`String.Iterator`.

More splitting required and the remaining material is quite unorganized,
but it's a start.

src/Init/Data/String/Basic.lean
@@ -7,6 +7,7 @@ module
 
 prelude
 public import Init.Data.String.Decode
+public import Init.Data.String.PosRaw
 import Init.Data.ByteArray.Lemmas
 
 public section
@@ -479,46 +480,6 @@ end
 
 namespace String
 
-instance : HSub String.Pos.Raw String String.Pos.Raw where
-  hSub p s := { byteIdx := p.byteIdx - s.utf8ByteSize }
-
-instance : HSub String.Pos.Raw Char String.Pos.Raw where
-  hSub p c := { byteIdx := p.byteIdx - c.utf8Size }
-
-@[export lean_string_pos_sub]
-def Pos.Internal.subImpl : String.Pos.Raw → String.Pos.Raw → String.Pos.Raw :=
-  fun p₁ p₂ => ⟨p₁.byteIdx - p₂.byteIdx⟩
-
-instance : HAdd String.Pos.Raw Char String.Pos.Raw where
-  hAdd p c := { byteIdx := p.byteIdx + c.utf8Size }
-
-instance : HAdd Char String.Pos.Raw String.Pos.Raw where
-  hAdd c p := { byteIdx := c.utf8Size + p.byteIdx }
-
-instance : HAdd String String.Pos.Raw String.Pos.Raw where
-  hAdd s p := { byteIdx := s.utf8ByteSize + p.byteIdx }
-
-instance : HAdd String.Pos.Raw String String.Pos.Raw where
-  hAdd p s := { byteIdx := p.byteIdx + s.utf8ByteSize }
-
-instance : LE String.Pos.Raw where
-  le p₁ p₂ := p₁.byteIdx ≤ p₂.byteIdx
-
-instance : LT String.Pos.Raw where
-  lt p₁ p₂ := p₁.byteIdx < p₂.byteIdx
-
-instance (p₁ p₂ : String.Pos.Raw) : Decidable (p₁ ≤ p₂) :=
-  inferInstanceAs (Decidable (p₁.byteIdx ≤ p₂.byteIdx))
-
-instance (p₁ p₂ : String.Pos.Raw) : Decidable (p₁ < p₂) :=
-  inferInstanceAs (Decidable (p₁.byteIdx < p₂.byteIdx))
-
-instance : Min String.Pos.Raw := minOfLe
-instance : Max String.Pos.Raw := maxOfLe
-
-theorem Pos.Raw.le_iff {i₁ i₂ : Pos.Raw} : i₁ ≤ i₂ ↔ i₁.byteIdx ≤ i₂.byteIdx := .rfl
-
-theorem Pos.Raw.lt_iff {i₁ i₂ : Pos.Raw} : i₁ < i₂ ↔ i₁.byteIdx < i₂.byteIdx := .rfl
 
 @[deprecated rawEndPos (since := "2025-10-20")]
 def endPos (s : String) : String.Pos.Raw :=
@@ -540,8 +501,6 @@ theorem byteIdx_endPos {s : String} : s.rawEndPos.byteIdx = s.utf8ByteSize := rf
 @[simp]
 theorem utf8ByteSize_ofByteArray {b : ByteArray} {h} :
     (String.ofByteArray b h).utf8ByteSize = b.size := rfl
-
-attribute [ext] String.Pos.Raw
 
 instance : LT String :=
   ⟨fun s₁ s₂ => s₁.data < s₂.data⟩
@@ -676,16 +635,13 @@ theorem Pos.Raw.isValid_iff_exists_append {s : String} {p : Pos.Raw} :
     simpa [ByteArray.extract_append_eq_left] using s₁.isValidUTF8
 
 @[simp]
-theorem Pos.Raw.byteIdx_zero : (0 : Pos.Raw).byteIdx = 0 := rfl
-
-@[simp]
 theorem Pos.Raw.isValid_zero {s : String} : (0 : Pos.Raw).IsValid s where
   le_rawEndPos := by simp [Pos.Raw.le_iff]
   isValidUTF8_extract_zero := by simp
 
 @[simp]
 theorem Pos.Raw.isValid_rawEndPos {s : String} : s.rawEndPos.IsValid s where
-  le_rawEndPos := by simp [Pos.Raw.le_iff]
+  le_rawEndPos := by simp
   isValidUTF8_extract_zero := by simp [← size_bytes, s.isValidUTF8]
 
 @[simp]
@@ -741,34 +697,6 @@ theorem Pos.Raw.isValid_singleton {c : Char} {p : Pos.Raw} :
   · rintro (rfl|hi)
     · exact ⟨0, by simp⟩
     · exact ⟨1, by simp [hi, ← singleton_eq_asString]⟩
-
-/--
-Returns the size of the byte slice delineated by the positions `lo` and `hi`.
--/
-@[expose, inline]
-def Pos.Raw.byteDistance (lo hi : Pos.Raw) : Nat :=
-  hi.byteIdx - lo.byteIdx
-
-theorem Pos.Raw.byteDistance_eq {lo hi : Pos.Raw} : lo.byteDistance hi = hi.byteIdx - lo.byteIdx :=
-  (rfl)
-
-@[simp]
-theorem Pos.Raw.byteIdx_sub_char {p : Pos.Raw} {c : Char} : (p - c).byteIdx = p.byteIdx - c.utf8Size := rfl
-
-@[simp]
-theorem Pos.Raw.byteIdx_sub_string {p : Pos.Raw} {s : String} : (p - s).byteIdx = p.byteIdx - s.utf8ByteSize := rfl
-
-@[simp]
-theorem Pos.Raw.byteIdx_add_string {p : Pos.Raw} {s : String} : (p + s).byteIdx = p.byteIdx + s.utf8ByteSize := rfl
-
-@[simp]
-theorem Pos.Raw.byteIdx_string_add {s : String} {p : Pos.Raw} : (s + p).byteIdx = s.utf8ByteSize + p.byteIdx := rfl
-
-@[simp]
-theorem Pos.Raw.byteIdx_add_char {p : Pos.Raw} {c : Char} : (p + c).byteIdx = p.byteIdx + c.utf8Size := rfl
-
-@[simp]
-theorem Pos.Raw.byteIdx_char_add {c : Char} {p : Pos.Raw} : (c + p).byteIdx = c.utf8Size + p.byteIdx := rfl
 
 theorem Pos.Raw.isValid_append {s t : String} {p : Pos.Raw} :
     p.IsValid (s ++ t) ↔ p.IsValid s ∨ (s.rawEndPos ≤ p ∧ (p - s).IsValid t) := by
@@ -850,25 +778,6 @@ where
     | cons a m ih =>
       rw [List.reverse_cons]
       exact append_singleton _ _ ih
-
-/--
-Accesses the indicated byte in the UTF-8 encoding of a string.
-
-At runtime, this function is implemented by efficient, constant-time code.
--/
-@[extern "lean_string_get_byte_fast", expose]
-def getUTF8Byte (s : @& String) (p : Pos.Raw) (h : p < s.rawEndPos) : UInt8 :=
-  s.bytes[p.byteIdx]
-
-@[deprecated getUTF8Byte (since := "2025-10-01"), extern "lean_string_get_byte_fast", expose]
-abbrev getUtf8Byte (s : String) (p : Pos.Raw) (h : p < s.rawEndPos) : UInt8 :=
-  s.getUTF8Byte p h
-
-@[simp]
-theorem rawEndPos_empty : "".rawEndPos = 0 := rfl
-
-@[deprecated rawEndPos_empty (since := "2025-10-20")]
-theorem endPos_empty : "".rawEndPos = 0 := rfl
 
 theorem Pos.Raw.isValid_iff_isUTF8FirstByte {s : String} {p : Pos.Raw} :
     p.IsValid s ↔ p = s.rawEndPos ∨ ∃ (h : p < s.rawEndPos), (s.getUTF8Byte p h).IsUTF8FirstByte := by
@@ -977,12 +886,6 @@ theorem _root_.ByteArray.IsValidUTF8.isUTF8FirstByte_getElem_zero {b : ByteArray
 theorem isUTF8FirstByte_getUTF8Byte_zero {b : String} {h} : (b.getUTF8Byte 0 h).IsUTF8FirstByte :=
   b.isValidUTF8.isUTF8FirstByte_getElem_zero _
 
-protected theorem Pos.Raw.le_trans {a b c : Pos.Raw} : a ≤ b → b ≤ c → a ≤ c := by
-  simpa [le_iff] using Nat.le_trans
-
-protected theorem Pos.Raw.lt_of_lt_of_le {a b c : Pos.Raw} : a < b → b ≤ c → a < c := by
-  simpa [le_iff, lt_iff] using Nat.lt_of_lt_of_le
-
 theorem Pos.Raw.isValidUTF8_extract_iff {s : String} (p₁ p₂ : Pos.Raw) (hle : p₁ ≤ p₂) (hle' : p₂ ≤ s.rawEndPos) :
     (s.bytes.extract p₁.byteIdx p₂.byteIdx).IsValidUTF8 ↔ p₁ = p₂ ∨ (p₁.IsValid s ∧ p₂.IsValid s) := by
   have hle'' : p₂.byteIdx ≤ s.bytes.size := by simpa [le_iff] using hle'
@@ -1019,7 +922,7 @@ theorem Pos.Raw.isValid_iff_isValidUTF8_extract_zero {s : String} {p : Pos.Raw} 
 theorem Pos.Raw.isValid_iff_isValidUTF8_extract_utf8ByteSize {s : String} {p : Pos.Raw} :
     p.IsValid s ↔ p ≤ s.rawEndPos ∧ (s.bytes.extract p.byteIdx s.utf8ByteSize).IsValidUTF8 := by
   refine ⟨fun h => ⟨h.le_rawEndPos, h.isValidUTF8_extract_utf8ByteSize⟩, fun ⟨h₁, h₂⟩ => ?_⟩
-  rw [← byteIdx_rawEndPos, isValidUTF8_extract_iff _ _ h₁ (by simp [le_iff])] at h₂
+  rw [← byteIdx_rawEndPos, isValidUTF8_extract_iff _ _ h₁ (by simp)] at h₂
   obtain (rfl|h₂) := h₂
   · simp
   · exact h₂.1
@@ -1105,7 +1008,7 @@ structure Slice where
   startInclusive_le_endExclusive : startInclusive ≤ endExclusive
 
 instance : Inhabited Slice where
-  default := ⟨"", "".startValidPos, "".startValidPos, by simp [ValidPos.le_iff, Pos.Raw.le_iff]⟩
+  default := ⟨"", "".startValidPos, "".startValidPos, by simp [ValidPos.le_iff]⟩
 
 /--
 Returns a slice that contains the entire string.
@@ -1153,40 +1056,6 @@ def Slice.rawEndPos (s : Slice) : Pos.Raw where
 
 @[simp]
 theorem Slice.byteIdx_rawEndPos {s : Slice} : s.rawEndPos.byteIdx = s.utf8ByteSize := (rfl)
-
-/--
-Offsets `p` by `offset` on the left. This is not an `HAdd` instance because it should be a
-relatively rare operation, so we use a name to make accidental use less likely. To offset a position
-by the size of a character character `c` or string `s`, you can use `c + p` resp. `s + p`.
-
-This should be seen as an operation that converts relative positions into absolute positions.
-
-See also `Pos.Raw.increaseBy`, which is an "advancing" operation.
--/
-@[expose, inline]
-def Pos.Raw.offsetBy (p : Pos.Raw) (offset : Pos.Raw) : Pos.Raw where
-  byteIdx := offset.byteIdx + p.byteIdx
-
-@[simp]
-theorem Pos.Raw.byteIdx_offsetBy {p : Pos.Raw} {offset : Pos.Raw} :
-    (p.offsetBy offset).byteIdx = offset.byteIdx + p.byteIdx := (rfl)
-
-/--
-Decreases `p` by `offset`. This is not an `HSub` instance because it should be a relatively
-rare operation, so we use a name to make accidental use less likely. To unoffset a position
-by the size of a character `c` or string `s`, you can use `p - c` resp. `p - s`.
-
-This should be seen as an operation that converts absolute positions into relative positions.
-
-See also `Pos.Raw.decreaseBy`, which is an "unadvancing" operation.
--/
-@[expose, inline]
-def Pos.Raw.unoffsetBy (p : Pos.Raw) (offset : Pos.Raw) : Pos.Raw where
-  byteIdx := p.byteIdx - offset.byteIdx
-
-@[simp]
-theorem Pos.Raw.byteIdx_unoffsetBy {p : Pos.Raw} {offset : Pos.Raw} :
-    (p.unoffsetBy offset).byteIdx = p.byteIdx - offset.byteIdx := (rfl)
 
 /-- Criterion for validity of positions in string slices. -/
 structure Pos.Raw.IsValidForSlice (s : Slice) (p : Pos.Raw) : Prop where
@@ -1300,7 +1169,7 @@ def Slice.startPos (s : Slice) : s.Pos where
   isValidForSlice := ⟨by simp [Pos.Raw.le_iff], by simpa using s.startInclusive.isValid⟩
 
 @[simp]
-theorem ByteString.Slice.offset_startPos {s : Slice} : s.startPos.offset = 0 := (rfl)
+theorem Slice.offset_startPos {s : Slice} : s.startPos.offset = 0 := (rfl)
 
 instance {s : Slice} : Inhabited s.Pos where
   default := s.startPos
@@ -1335,10 +1204,10 @@ theorem Pos.Raw.offsetBy_sliceRawEndPos_right {p : Pos.Raw} {s : Slice} :
 @[inline, expose]
 def Slice.endPos (s : Slice) : s.Pos where
   offset := s.rawEndPos
-  isValidForSlice := ⟨by simp [Pos.Raw.le_iff], by simpa using s.endExclusive.isValid⟩
+  isValidForSlice := ⟨by simp, by simpa using s.endExclusive.isValid⟩
 
 @[simp]
-theorem ByteString.Slice.offset_endPos {s : Slice} : s.endPos.offset = s.rawEndPos := (rfl)
+theorem Slice.offset_endPos {s : Slice} : s.endPos.offset = s.rawEndPos := (rfl)
 
 instance {s : Slice} : LE s.Pos where
   le l r := l.offset ≤ r.offset
@@ -1576,11 +1445,6 @@ theorem Slice.utf8ByteSize_replaceStartEnd {s : Slice} {newStart newEnd : s.Pos}
   simp [utf8ByteSize_eq, Pos.Raw.byteDistance_eq]
   omega
 
-theorem Pos.Raw.offsetBy_assoc {p q r : Pos.Raw} :
-    (p.offsetBy q).offsetBy r = p.offsetBy (q.offsetBy r) := by
-  ext
-  simp [Nat.add_assoc]
-
 theorem Pos.Raw.isValidForSlice_replaceStart {s : Slice} {p : s.Pos} {off : Pos.Raw} :
     off.IsValidForSlice (s.replaceStart p) ↔ (off.offsetBy p.offset).IsValidForSlice s := by
   refine ⟨fun ⟨h₁, h₂⟩ => ⟨?_, ?_⟩, fun ⟨h₁, h₂⟩ => ⟨?_, ?_⟩⟩
@@ -1754,10 +1618,6 @@ theorem utf8ByteSize_eq_zero_iff {s : String} : s.utf8ByteSize = 0 ↔ s = "" :=
   refine ⟨fun h => ?_, fun h => h ▸ utf8ByteSize_empty⟩
   simpa [← bytes_inj, ← ByteArray.size_eq_zero_iff] using h
 
-@[simp]
-theorem Pos.Raw.eq_zero_iff {p : Pos.Raw} : p = 0 ↔ p.byteIdx = 0 :=
-  Pos.Raw.ext_iff
-
 theorem rawEndPos_eq_zero_iff {b : String} : b.rawEndPos = 0 ↔ b = "" := by
   simp
 
@@ -1858,7 +1718,7 @@ theorem Slice.Pos.get_toCopy {s : Slice} {pos : s.Pos} (h) :
     pos.toCopy.get h = pos.get (by rintro rfl; simp at h) := by
   rw [ValidPos.get, Slice.Pos.get_eq_utf8DecodeChar, Slice.Pos.get_eq_utf8DecodeChar]
   simp only [str_toSlice, bytes_copy, startInclusive_toSlice, startValidPos_copy, offset_toCopy,
-    ByteString.Slice.offset_startPos, Pos.Raw.byteIdx_zero, ValidPos.offset_toSlice, Nat.zero_add]
+    Slice.offset_startPos, Pos.Raw.byteIdx_zero, ValidPos.offset_toSlice, Nat.zero_add]
   rw [ByteArray.utf8DecodeChar_eq_utf8DecodeChar_extract]
   conv => lhs; congr; rw [ByteArray.extract_extract]
   conv => rhs; rw [ByteArray.utf8DecodeChar_eq_utf8DecodeChar_extract]
@@ -1887,16 +1747,6 @@ def Slice.Pos.ofReplaceStart {s : Slice} {p₀ : s.Pos} (pos : (s.replaceStart p
 theorem Slice.Pos.offset_ofReplaceStart {s : Slice} {p₀ : s.Pos} {pos : (s.replaceStart p₀).Pos} :
     (ofReplaceStart pos).offset = pos.offset.offsetBy p₀.offset := (rfl)
 
-theorem Pos.Raw.offsetBy_unoffsetBy_of_le {p : Pos.Raw} {q : Pos.Raw} (h : q ≤ p) :
-    (p.unoffsetBy q).offsetBy q = p := by
-  ext
-  simp_all [le_iff]
-
-@[simp]
-theorem Pos.Raw.unoffsetBy_offsetBy {p q : Pos.Raw} : (p.offsetBy q).unoffsetBy q = p := by
-  ext
-  simp
-
 /-- Given a position in `s` that is at least `p₀`, obtain the corresponding position in
 `s.replaceStart p₀`. -/
 @[inline]
@@ -1909,11 +1759,6 @@ def Slice.Pos.toReplaceStart {s : Slice} (p₀ : s.Pos) (pos : s.Pos) (h : p₀ 
 @[simp]
 theorem Slice.Pos.offset_toReplaceStart {s : Slice} {p₀ : s.Pos} {pos : s.Pos} {h} :
     (toReplaceStart p₀ pos h).offset = pos.offset.unoffsetBy p₀.offset := (rfl)
-
-@[simp]
-theorem Pos.Raw.offsetBy_zero_left {p : Pos.Raw} : (0 : Pos.Raw).offsetBy p = p := by
-  ext
-  simp
 
 @[simp]
 theorem Slice.Pos.ofReplaceStart_startPos {s : Slice} {pos : s.Pos} :
@@ -1970,44 +1815,6 @@ theorem ValidPos.utf8ByteSize_byte {s : String} {pos : s.ValidPos} {h : pos ≠ 
     (pos.byte h).utf8ByteSize pos.isUTF8FirstByte_byte = (pos.get h).utf8Size :=
   Slice.Pos.utf8ByteSize_byte
 
-/--
-Advances `p` by `n` bytes. This is not an `HAdd` instance because it should be a relatively
-rare operation, so we use a name to make accidental use less likely. To add the size of a
-character `c` or string `s` to a raw position `p`, you can use `p + c` resp. `p + s`.
-
-This should be seen as an "advance" or "skip".
-
-See also `Pos.Raw.offsetBy`, which turns relative positions into absolute positions.
--/
-@[expose, inline]
-def Pos.Raw.increaseBy (p : Pos.Raw) (n : Nat) : Pos.Raw where
-  byteIdx := p.byteIdx + n
-
-@[simp]
-theorem Pos.Raw.byteIdx_increaseBy {p : Pos.Raw} {n : Nat} :
-    (p.increaseBy n).byteIdx = p.byteIdx + n := (rfl)
-
-/--
-Move the position `p` back by `n` bytes. This is not an `HSub` instance because it should be a
-relatively rare operation, so we use a name to make accidental use less likely. To remove the size
-of a character `c` or string `s` from a raw position `p`, you can use `p - c` resp. `p - s`.
-
-This should be seen as the inverse of an "advance" or "skip".
-
-See also `Pos.Raw.unoffsetBy`, which turns absolute positions into relative positions.
--/
-@[expose, inline]
-def Pos.Raw.decreaseBy (p : Pos.Raw) (n : Nat) : Pos.Raw where
-  byteIdx := p.byteIdx - n
-
-@[simp]
-theorem Pos.Raw.byteIdx_decreaseBy {p : Pos.Raw} {n : Nat} :
-    (p.decreaseBy n).byteIdx = p.byteIdx - n := (rfl)
-
-theorem Pos.Raw.increaseBy_charUtf8Size {p : Pos.Raw} {c : Char} :
-    p.increaseBy c.utf8Size = p + c := by
-  simp [Pos.Raw.ext_iff]
-
 /-- Advances a valid position on a slice to the next valid position, given a proof that the
 position is not the past-the-end position, which guarantees that such a position exists. -/
 @[expose]
@@ -2048,22 +1855,6 @@ theorem Slice.Pos.byteIdx_offset_next {s : Slice} {pos : s.Pos} {h : pos ≠ s.e
 theorem Slice.Pos.lt_next {s : Slice} {pos : s.Pos} {h : pos ≠ s.endPos} :
     pos < pos.next h := by
   simp [Pos.lt_iff, Pos.Raw.lt_iff, Char.utf8Size_pos]
-
-/-- Increases the byte offset of the position by `1`. Not to be confused with `ValidPos.next`. -/
-@[inline, expose]
-def Pos.Raw.inc (p : Pos.Raw) : Pos.Raw :=
-  ⟨p.byteIdx + 1⟩
-
-@[simp]
-theorem Pos.Raw.byteIdx_inc {p : Pos.Raw} : p.inc.byteIdx = p.byteIdx + 1 := (rfl)
-
-/-- Decreases the byte offset of the position by `1`. Not to be confused with `ValidPos.prev`. -/
-@[inline, expose]
-def Pos.Raw.dec (p : Pos.Raw) : Pos.Raw :=
-  ⟨p.byteIdx - 1⟩
-
-@[simp]
-theorem Pos.Raw.byteIdx_dec {p : Pos.Raw} : p.dec.byteIdx = p.byteIdx - 1 := (rfl)
 
 @[inline, expose]
 def Slice.Pos.prevAux {s : Slice} (pos : s.Pos) (h : pos ≠ s.startPos) : String.Pos.Raw :=
@@ -2247,15 +2038,6 @@ where
     simp only [Pos.Raw.lt_iff, byteIdx_rawEndPos, utf8ByteSize_eq, Pos.Raw.byteIdx_inc] at h ⊢
     omega
 
-@[simp]
-theorem Pos.Raw.le_refl {p : Pos.Raw} : p ≤ p := by simp [le_iff]
-
-theorem Pos.Raw.lt_inc {p : Pos.Raw} : p < p.inc := by simp [lt_iff]
-
-theorem Pos.Raw.le_of_lt {p q : Pos.Raw} : p < q → p ≤ q := by simpa [lt_iff, le_iff] using Nat.le_of_lt
-
-theorem Pos.Raw.inc_le {p q : Pos.Raw} : p.inc ≤ q ↔ p < q := by simpa [lt_iff, le_iff] using Nat.succ_le
-
 private theorem Slice.le_offset_findNextPosGo {s : Slice} {o : String.Pos.Raw} (h : o ≤ s.rawEndPos) :
     o ≤ (findNextPos.go s o).offset := by
   fun_induction findNextPos.go with
@@ -2285,9 +2067,6 @@ theorem Slice.Pos.prevAuxGo_le_self {s : Slice} {p : Nat} {h : p < s.utf8ByteSiz
 where
   elim (P : String.Pos.Raw → Prop) {h : False} : P h.elim := h.elim
 
-theorem Pos.Raw.lt_of_le_of_lt {a b c : Pos.Raw} : a ≤ b → b < c → a < c := by
-  simpa [le_iff, lt_iff] using Nat.lt_of_le_of_lt
-
 theorem Slice.Pos.prevAux_lt_self {s : Slice} {p : s.Pos} {h} : p.prevAux h < p.offset := by
   rw [prevAux]
   refine Pos.Raw.lt_of_le_of_lt prevAuxGo_le_self ?_
@@ -2296,9 +2075,6 @@ theorem Slice.Pos.prevAux_lt_self {s : Slice} {p : s.Pos} {h} : p.prevAux h < p.
 
 theorem Slice.Pos.prevAux_lt_rawEndPos {s : Slice} {p : s.Pos} {h} : p.prevAux h < s.rawEndPos :=
   Pos.Raw.lt_of_lt_of_le prevAux_lt_self p.isValidForSlice.le_utf8ByteSize
-
-theorem Pos.Raw.ne_of_lt {a b : Pos.Raw} : a < b → a ≠ b := by
-  simpa [lt_iff, Pos.Raw.ext_iff] using Nat.ne_of_lt
 
 theorem Slice.Pos.prev_ne_endPos {s : Slice} {p : s.Pos} {h} : p.prev h ≠ s.endPos := by
   simpa [Pos.ext_iff, prev] using Pos.Raw.ne_of_lt prevAux_lt_rawEndPos
@@ -2803,17 +2579,6 @@ def next' (s : @& String) (p : @& Pos.Raw) (h : ¬ p.atEnd s) : Pos.Raw :=
   let c := p.get s
   p + c
 
-@[deprecated Pos.Raw.lt_iff (since := "2025-10-10")]
-theorem pos_lt_eq (p₁ p₂ : Pos.Raw) : (p₁ < p₂) = (p₁.1 < p₂.1) :=
-  propext Pos.Raw.lt_iff
-
-@[deprecated Pos.Raw.byteIdx_add_char (since := "2025-10-10")]
-theorem pos_add_char (p : Pos.Raw) (c : Char) : (p + c).byteIdx = p.byteIdx + c.utf8Size :=
-  Pos.Raw.byteIdx_add_char
-
-protected theorem Pos.Raw.ne_zero_of_lt : {a b : Pos.Raw} → a < b → b ≠ 0
-  | _, _, hlt, rfl => Nat.not_lt_zero _ hlt
-
 theorem Pos.Raw.lt_next (s : String) (i : Pos.Raw) : i < i.next s :=
   Nat.add_lt_add_left (Char.utf8Size_pos _) _
 
@@ -2928,16 +2693,6 @@ Examples:
 -/
 @[inline] def revFind (s : String) (p : Char → Bool) : Option Pos.Raw :=
   revFindAux s p s.rawEndPos
-
-/--
-Returns either `p₁` or `p₂`, whichever has the least byte index.
--/
-abbrev Pos.Raw.min (p₁ p₂ : Pos.Raw) : Pos.Raw :=
-  { byteIdx := p₁.byteIdx.min p₂.byteIdx }
-
-@[export lean_string_pos_min]
-def Pos.Raw.Internal.minImpl (p₁ p₂ : Pos.Raw) : Pos.Raw :=
-  Pos.Raw.min p₁ p₂
 
 /--
 Returns the first position where the two strings differ.
@@ -3163,189 +2918,6 @@ where go (acc : String) (s : String) : List String → String
 def Internal.intercalateImpl (s : String) : List String → String :=
   String.intercalate s
 
-/--
-An iterator over the characters (Unicode code points) in a `String`. Typically created by
-`String.iter`.
-
-String iterators pair a string with a valid byte index. This allows efficient character-by-character
-processing of strings while avoiding the need to manually ensure that byte indices are used with the
-correct strings.
-
-An iterator is *valid* if the position `i` is *valid* for the string `s`, meaning `0 ≤ i ≤ s.rawEndPos`
-and `i` lies on a UTF8 byte boundary. If `i = s.rawEndPos`, the iterator is at the end of the string.
-
-Most operations on iterators return unspecified values if the iterator is not valid. The functions
-in the `String.Iterator` API rule out the creation of invalid iterators, with two exceptions:
-- `Iterator.next iter` is invalid if `iter` is already at the end of the string (`iter.atEnd` is
-  `true`), and
-- `Iterator.forward iter n`/`Iterator.nextn iter n` is invalid if `n` is strictly greater than the
-  number of remaining characters.
--/
-structure Iterator where
-  /-- The string being iterated over. -/
-  s : String
-  /-- The current UTF-8 byte position in the string `s`.
-
-  This position is not guaranteed to be valid for the string. If the position is not valid, then the
-  current character is `(default : Char)`, similar to `String.get` on an invalid position.
-  -/
-  i : Pos.Raw
-  deriving DecidableEq, Inhabited
-
-/-- Creates an iterator at the beginning of the string. -/
-@[inline] def mkIterator (s : String) : Iterator :=
-  ⟨s, 0⟩
-
-@[inherit_doc mkIterator]
-abbrev iter := mkIterator
-
-/--
-The size of a string iterator is the number of bytes remaining.
-
-Recursive functions that iterate towards the end of a string will typically decrease this measure.
--/
-instance : SizeOf String.Iterator where
-  sizeOf i := i.1.utf8ByteSize - i.2.byteIdx
-
-theorem Iterator.sizeOf_eq (i : String.Iterator) : sizeOf i = i.1.utf8ByteSize - i.2.byteIdx :=
-  rfl
-
-namespace Iterator
-@[inline, inherit_doc Iterator.s]
-def toString := Iterator.s
-
-/--
-The number of UTF-8 bytes remaining in the iterator.
--/
-@[inline] def remainingBytes : Iterator → Nat
-  | ⟨s, i⟩ => s.rawEndPos.byteIdx - i.byteIdx
-
-@[inline, inherit_doc Iterator.i]
-def pos := Iterator.i
-
-/--
-Gets the character at the iterator's current position.
-
-A run-time bounds check is performed. Use `String.Iterator.curr'` to avoid redundant bounds checks.
-
-If the position is invalid, returns `(default : Char)`.
--/
-@[inline] def curr : Iterator → Char
-  | ⟨s, i⟩ => i.get s
-
-/--
-Moves the iterator's position forward by one character, unconditionally.
-
-It is only valid to call this function if the iterator is not at the end of the string (i.e.
-if `Iterator.atEnd` is `false`); otherwise, the resulting iterator will be invalid.
--/
-@[inline] def next : Iterator → Iterator
-  | ⟨s, i⟩ => ⟨s, i.next s⟩
-
-/--
-Moves the iterator's position backward by one character, unconditionally.
-
-The position is not changed if the iterator is at the beginning of the string.
--/
-@[inline] def prev : Iterator → Iterator
-  | ⟨s, i⟩ => ⟨s, i.prev s⟩
-
-/--
-Checks whether the iterator is past its string's last character.
--/
-@[inline] def atEnd : Iterator → Bool
-  | ⟨s, i⟩ => i.byteIdx ≥ s.rawEndPos.byteIdx
-
-/--
-Checks whether the iterator is at or before the string's last character.
--/
-@[inline] def hasNext : Iterator → Bool
-  | ⟨s, i⟩ => i.byteIdx < s.rawEndPos.byteIdx
-
-/--
-Checks whether the iterator is after the beginning of the string.
--/
-@[inline] def hasPrev : Iterator → Bool
-  | ⟨_, i⟩ => i.byteIdx > 0
-
-/--
-Gets the character at the iterator's current position.
-
-The proof of `it.hasNext` ensures that there is, in fact, a character at the current position. This
-function is faster that `String.Iterator.curr` due to avoiding a run-time bounds check.
--/
-@[inline] def curr' (it : Iterator) (h : it.hasNext) : Char :=
-  match it with
-  | ⟨s, i⟩ => i.get' s (by simpa only [hasNext, rawEndPos, decide_eq_true_eq, Pos.Raw.atEnd, ge_iff_le, Nat.not_le] using h)
-
-/--
-Moves the iterator's position forward by one character, unconditionally.
-
-The proof of `it.hasNext` ensures that there is, in fact, a position that's one character forwards.
-This function is faster that `String.Iterator.next` due to avoiding a run-time bounds check.
--/
-@[inline] def next' (it : Iterator) (h : it.hasNext) : Iterator :=
-  match it with
-  | ⟨s, i⟩ => ⟨s, i.next' s (by simpa only [hasNext, rawEndPos, decide_eq_true_eq, Pos.Raw.atEnd, ge_iff_le, Nat.not_le] using h)⟩
-
-/--
-Replaces the current character in the string.
-
-Does nothing if the iterator is at the end of the string. If both the replacement character and the
-replaced character are 7-bit ASCII characters and the string is not shared, then it is updated
-in-place and not copied.
--/
-@[inline] def setCurr : Iterator → Char → Iterator
-  | ⟨s, i⟩, c => ⟨i.set s c, i⟩
-
-/--
-Moves the iterator's position to the end of the string, just past the last character.
--/
-@[inline] def toEnd : Iterator → Iterator
-  | ⟨s, _⟩ => ⟨s, s.rawEndPos⟩
-
-/--
-Extracts the substring between the positions of two iterators. The first iterator's position is the
-start of the substring, and the second iterator's position is the end.
-
-Returns the empty string if the iterators are for different strings, or if the position of the first
-iterator is past the position of the second iterator.
--/
-@[inline] def extract : Iterator → Iterator → String
-  | ⟨s₁, b⟩, ⟨s₂, e⟩ =>
-    if s₁ ≠ s₂ || b > e then ""
-    else b.extract s₁ e
-
-/--
-Moves the iterator's position forward by the specified number of characters.
-
-The resulting iterator is only valid if the number of characters to skip is less than or equal
-to the number of characters left in the iterator.
--/
-def forward : Iterator → Nat → Iterator
-  | it, 0   => it
-  | it, n+1 => forward it.next n
-
-/--
-The remaining characters in an iterator, as a string.
--/
-@[inline] def remainingToString : Iterator → String
-  | ⟨s, i⟩ => i.extract s s.rawEndPos
-
-@[inherit_doc forward]
-def nextn : Iterator → Nat → Iterator
-  | it, 0   => it
-  | it, i+1 => nextn it.next i
-
-/--
-Moves the iterator's position back by the specified number of characters, stopping at the beginning
-of the string.
--/
-def prevn : Iterator → Nat → Iterator
-  | it, 0   => it
-  | it, i+1 => prevn it.prev i
-
-end Iterator
 
 def offsetOfPosAux (s : String) (pos : Pos.Raw) (i : Pos.Raw) (offset : Nat) : Nat :=
   if i >= pos then offset
@@ -3664,739 +3236,9 @@ def findLineStart (s : String) (pos : String.Pos.Raw) : String.Pos.Raw :=
 
 end String
 
-namespace Substring
-
-/--
-Checks whether a substring is empty.
-
-A substring is empty if its start and end positions are the same.
--/
-@[inline] def isEmpty (ss : Substring) : Bool :=
-  ss.bsize == 0
-
-@[export lean_substring_isempty]
-def Internal.isEmptyImpl (ss : Substring) : Bool :=
-  Substring.isEmpty ss
-
-/--
-Copies the region of the underlying string pointed to by a substring into a fresh string.
--/
-@[inline] def toString : Substring → String
-  | ⟨s, b, e⟩ => b.extract s e
-
-@[export lean_substring_tostring]
-def Internal.toStringImpl : Substring → String :=
-  Substring.toString
-
-/--
-Returns an iterator into the underlying string, at the substring's starting position. The ending
-position is discarded, so the iterator alone cannot be used to determine whether its current
-position is within the original substring.
--/
-@[inline] def toIterator : Substring → String.Iterator
-  | ⟨s, b, _⟩ => ⟨s, b⟩
-
-/--
-Returns the character at the given position in the substring.
-
-The position is relative to the substring, rather than the underlying string, and no bounds checking
-is performed with respect to the substring's end position. If the relative position is not a valid
-position in the underlying string, the fallback value `(default : Char)`, which is `'A'`, is
-returned.  Does not panic.
--/
-@[inline] def get : Substring → String.Pos.Raw → Char
-  | ⟨s, b, _⟩, p => (p.offsetBy b).get s
-
-@[export lean_substring_get]
-def Internal.getImpl : Substring → String.Pos.Raw → Char :=
-  Substring.get
-
-/--
-Returns the next position in a substring after the given position. If the position is at the end of
-the substring, it is returned unmodified.
-
-Both the input position and the returned position are interpreted relative to the substring's start
-position, not the underlying string.
--/
-@[inline] def next : Substring → String.Pos.Raw → String.Pos.Raw
-  | ⟨s, b, e⟩, p =>
-    let absP := p.offsetBy b
-    if absP = e then p else { byteIdx := (absP.next s).byteIdx - b.byteIdx }
-
-theorem lt_next (s : Substring) (i : String.Pos.Raw) (h : i.1 < s.bsize) :
-    i.1 < (s.next i).1 := by
-  simp [next]; rw [if_neg ?a]
-  case a =>
-    refine mt (congrArg String.Pos.Raw.byteIdx) (Nat.ne_of_lt ?_)
-    exact (Nat.add_comm .. ▸ Nat.add_lt_of_lt_sub h :)
-  apply Nat.lt_sub_of_add_lt
-  rw [Nat.add_comm]; apply String.Pos.Raw.lt_next
-
-/--
-Returns the previous position in a substring, just prior to the given position. If the position is
-at the beginning of the substring, it is returned unmodified.
-
-Both the input position and the returned position are interpreted relative to the substring's start
-position, not the underlying string.
--/
-@[inline] def prev : Substring → String.Pos.Raw → String.Pos.Raw
-  | ⟨s, b, _⟩, p =>
-    let absP := p.offsetBy b
-    if absP = b then p else { byteIdx := (absP.prev s).byteIdx - b.byteIdx }
-
-@[export lean_substring_prev]
-def Internal.prevImpl : Substring → String.Pos.Raw → String.Pos.Raw :=
-  Substring.prev
-
-/--
-Returns the position that's the specified number of characters forward from the given position in a
-substring. If the end position of the substring is reached, it is returned.
-
-Both the input position and the returned position are interpreted relative to the substring's start
-position, not the underlying string.
--/
-def nextn : Substring → Nat → String.Pos.Raw → String.Pos.Raw
-  | _,  0,   p => p
-  | ss, i+1, p => ss.nextn i (ss.next p)
-
-/--
-Returns the position that's the specified number of characters prior to the given position in a
-substring. If the start position of the substring is reached, it is returned.
-
-Both the input position and the returned position are interpreted relative to the substring's start
-position, not the underlying string.
--/
-def prevn : Substring → Nat → String.Pos.Raw → String.Pos.Raw
-  | _,  0,   p => p
-  | ss, i+1, p => ss.prevn i (ss.prev p)
-
-/--
-Returns the first character in the substring.
-
-If the substring is empty, but the substring's start position is a valid position in the underlying
-string, then the character at the start position is returned. If the substring's start position is
-not a valid position in the string, the fallback value `(default : Char)`, which is `'A'`, is
-returned.  Does not panic.
--/
-@[inline, expose] def front (s : Substring) : Char :=
-  s.get 0
-
-@[export lean_substring_front]
-def Internal.frontImpl : Substring → Char :=
-  Substring.front
-
-/--
-Returns the substring-relative position of the first occurrence of `c` in `s`, or `s.bsize` if `c`
-doesn't occur.
--/
-@[inline] def posOf (s : Substring) (c : Char) : String.Pos.Raw :=
-  match s with
-  | ⟨s, b, e⟩ => { byteIdx := (String.posOfAux s c e b).byteIdx - b.byteIdx }
-
-/--
-Removes the specified number of characters (Unicode code points) from the beginning of a substring
-by advancing its start position.
-
-If the substring's end position is reached, the start position is not advanced past it.
--/
-@[inline] def drop : Substring → Nat → Substring
-  | ss@⟨s, b, e⟩, n => ⟨s, (ss.nextn n 0).offsetBy b, e⟩
-
-@[export lean_substring_drop]
-def Internal.dropImpl : Substring → Nat → Substring :=
-  Substring.drop
-
-/--
-Removes the specified number of characters (Unicode code points) from the end of a substring
-by moving its end position towards its start position.
-
-If the substring's start position is reached, the end position is not retracted past it.
--/
-@[inline] def dropRight : Substring → Nat → Substring
-  | ss@⟨s, b, _⟩, n => ⟨s, b, (ss.prevn n ⟨ss.bsize⟩).offsetBy b⟩
-
-/--
-Retains only the specified number of characters (Unicode code points) at the beginning of a
-substring, by moving its end position towards its start position.
-
-If the substring's start position is reached, the end position is not retracted past it.
--/
-@[inline] def take : Substring → Nat → Substring
-  | ss@⟨s, b, _⟩, n => ⟨s, b, (ss.nextn n 0).offsetBy b⟩
-
-/--
-Retains only the specified number of characters (Unicode code points) at the end of a substring, by
-moving its start position towards its end position.
-
-If the substring's end position is reached, the start position is not advanced past it.
--/
-@[inline] def takeRight : Substring → Nat → Substring
-  | ss@⟨s, b, e⟩, n => ⟨s, (ss.prevn n ⟨ss.bsize⟩).offsetBy b, e⟩
-
-/--
-Checks whether a position in a substring is precisely equal to its ending position.
-
-The position is understood relative to the substring's starting position, rather than the underlying
-string's starting position.
--/
-@[inline] def atEnd : Substring → String.Pos.Raw → Bool
-  | ⟨_, b, e⟩, p => p.offsetBy b == e
-
-/--
-Returns the region of the substring delimited by the provided start and stop positions, as a
-substring. The positions are interpreted with respect to the substring's start position, rather than
-the underlying string.
-
-If the resulting substring is empty, then the resulting substring is a substring of the empty string
-`""`. Otherwise, the underlying string is that of the input substring with the beginning and end
-positions adjusted.
--/
-@[inline] def extract : Substring → String.Pos.Raw → String.Pos.Raw → Substring
-  | ⟨s, b, e⟩, b', e' => if b' ≥ e' then ⟨"", 0, 0⟩ else ⟨s, e.min (b'.offsetBy b), e.min (e'.offsetBy b)⟩
-
-@[export lean_substring_extract]
-def Internal.extractImpl : Substring → String.Pos.Raw → String.Pos.Raw → Substring :=
-  Substring.extract
-
-/--
-Splits a substring `s` on occurrences of the separator string `sep`. The default separator is `" "`.
-
-When `sep` is empty, the result is `[s]`. When `sep` occurs in overlapping patterns, the first match
-is taken. There will always be exactly `n+1` elements in the returned list if there were `n`
-non-overlapping matches of `sep` in the string. The separators are not included in the returned
-substrings, which are all substrings of `s`'s string.
--/
-def splitOn (s : Substring) (sep : String := " ") : List Substring :=
-  if sep == "" then
-    [s]
-  else
-    let rec loop (b i j : String.Pos.Raw) (r : List Substring) : List Substring :=
-      if h : i.byteIdx < s.bsize then
-        have := Nat.sub_lt_sub_left h (lt_next s i h)
-        if s.get i == j.get sep then
-          let i := s.next i
-          let j := j.next sep
-          if j.atEnd sep then
-            loop i i 0 (s.extract b (i.unoffsetBy j) :: r)
-          else
-            loop b i j r
-        else
-          loop b (s.next i) 0 r
-      else
-        let r := if j.atEnd sep then
-          "".toSubstring :: s.extract b (i.unoffsetBy j) :: r
-        else
-          s.extract b i :: r
-        r.reverse
-      termination_by s.bsize - i.1
-    loop 0 0 0 []
-
-/--
-Folds a function over a substring from the left, accumulating a value starting with `init`. The
-accumulated value is combined with each character in order, using `f`.
--/
-@[inline] def foldl {α : Type u} (f : α → Char → α) (init : α) (s : Substring) : α :=
-  match s with
-  | ⟨s, b, e⟩ => String.foldlAux f s e b init
-
-/--
-Folds a function over a substring from the right, accumulating a value starting with `init`. The
-accumulated value is combined with each character in reverse order, using `f`.
--/
-@[inline] def foldr {α : Type u} (f : Char → α → α) (init : α) (s : Substring) : α :=
-  match s with
-  | ⟨s, b, e⟩ => String.foldrAux f init s e b
-
-/--
-Checks whether the Boolean predicate `p` returns `true` for any character in a substring.
-
-Short-circuits at the first character for which `p` returns `true`.
--/
-@[inline] def any (s : Substring) (p : Char → Bool) : Bool :=
-  match s with
-  | ⟨s, b, e⟩ => String.anyAux s e p b
-
-/--
-Checks whether the Boolean predicate `p` returns `true` for every character in a substring.
-
-Short-circuits at the first character for which `p` returns `false`.
--/
-@[inline] def all (s : Substring) (p : Char → Bool) : Bool :=
-  !s.any (fun c => !p c)
-
-@[export lean_substring_all]
-def Internal.allImpl (s : Substring) (p : Char → Bool) : Bool :=
-  Substring.all s p
-
-/--
-Checks whether a substring contains the specified character.
--/
-@[inline] def contains (s : Substring) (c : Char) : Bool :=
-  s.any (fun a => a == c)
-
-@[specialize] def takeWhileAux (s : String) (stopPos : String.Pos.Raw) (p : Char → Bool) (i : String.Pos.Raw) : String.Pos.Raw :=
-  if h : i < stopPos then
-    if p (i.get s) then
-      have := Nat.sub_lt_sub_left h (String.Pos.Raw.lt_next s i)
-      takeWhileAux s stopPos p (i.next s)
-    else i
-  else i
-termination_by stopPos.1 - i.1
-
-/--
-Retains only the longest prefix of a substring in which a Boolean predicate returns `true` for all
-characters by moving the substring's end position towards its start position.
--/
-@[inline] def takeWhile : Substring → (Char → Bool) → Substring
-  | ⟨s, b, e⟩, p =>
-    let e := takeWhileAux s e p b;
-    ⟨s, b, e⟩
-
-@[export lean_substring_takewhile]
-def Internal.takeWhileImpl : Substring → (Char → Bool) → Substring :=
-  Substring.takeWhile
-
-/--
-Removes the longest prefix of a substring in which a Boolean predicate returns `true` for all
-characters by moving the substring's start position. The start position is moved to the position of
-the first character for which the predicate returns `false`, or to the substring's end position if
-the predicate always returns `true`.
--/
-@[inline] def dropWhile : Substring → (Char → Bool) → Substring
-  | ⟨s, b, e⟩, p =>
-    let b := takeWhileAux s e p b;
-    ⟨s, b, e⟩
-
-@[specialize] def takeRightWhileAux (s : String) (begPos : String.Pos.Raw) (p : Char → Bool) (i : String.Pos.Raw) : String.Pos.Raw :=
-  if h : begPos < i then
-    have := String.Pos.Raw.prev_lt_of_pos s i <| mt (congrArg String.Pos.Raw.byteIdx) <|
-      Ne.symm <| Nat.ne_of_lt <| Nat.lt_of_le_of_lt (Nat.zero_le _) h
-    let i' := i.prev s
-    let c  := i'.get s
-    if !p c then i
-    else takeRightWhileAux s begPos p i'
-  else i
-termination_by i.1
-
-/--
-Retains only the longest suffix of a substring in which a Boolean predicate returns `true` for all
-characters by moving the substring's start position towards its end position.
--/
-@[inline] def takeRightWhile : Substring → (Char → Bool) → Substring
-  | ⟨s, b, e⟩, p =>
-    let b := takeRightWhileAux s b p e
-    ⟨s, b, e⟩
-
-/--
-Removes the longest suffix of a substring in which a Boolean predicate returns `true` for all
-characters by moving the substring's end position. The end position is moved just after the position
-of the last character for which the predicate returns `false`, or to the substring's start position
-if the predicate always returns `true`.
--/
-@[inline] def dropRightWhile : Substring → (Char → Bool) → Substring
-  | ⟨s, b, e⟩, p =>
-    let e := takeRightWhileAux s b p e
-    ⟨s, b, e⟩
-
-/--
-Removes leading whitespace from a substring by moving its start position to the first non-whitespace
-character, or to its end position if there is no non-whitespace character.
-
-“Whitespace” is defined as characters for which `Char.isWhitespace` returns `true`.
--/
-@[inline] def trimLeft (s : Substring) : Substring :=
-  s.dropWhile Char.isWhitespace
-
-/--
-Removes trailing whitespace from a substring by moving its end position to the last non-whitespace
-character, or to its start position if there is no non-whitespace character.
-
-“Whitespace” is defined as characters for which `Char.isWhitespace` returns `true`.
--/
-@[inline] def trimRight (s : Substring) : Substring :=
-  s.dropRightWhile Char.isWhitespace
-
-/--
-Removes leading and trailing whitespace from a substring by first moving its start position to the
-first non-whitespace character, and then moving its end position to the last non-whitespace
-character.
-
-If the substring consists only of whitespace, then the resulting substring's start position is moved
-to its end position.
-
-“Whitespace” is defined as characters for which `Char.isWhitespace` returns `true`.
-
-Examples:
- * `" red green blue ".toSubstring.trim.toString = "red green blue"`
- * `" red green blue ".toSubstring.trim.startPos = ⟨1⟩`
- * `" red green blue ".toSubstring.trim.stopPos = ⟨15⟩`
- * `"     ".toSubstring.trim.startPos = ⟨5⟩`
--/
-@[inline] def trim : Substring → Substring
-  | ⟨s, b, e⟩ =>
-    let b := takeWhileAux s e Char.isWhitespace b
-    let e := takeRightWhileAux s b Char.isWhitespace e
-    ⟨s, b, e⟩
-
-/--
-Checks whether the substring can be interpreted as the decimal representation of a natural number.
-
-A substring can be interpreted as a decimal natural number if it is not empty and all the characters
-in it are digits.
-
-Use `Substring.toNat?` to convert such a substring to a natural number.
--/
-@[inline] def isNat (s : Substring) : Bool :=
-  !s.isEmpty && s.all fun c => c.isDigit
-
-/--
-Checks whether the substring can be interpreted as the decimal representation of a natural number,
-returning the number if it can.
-
-A substring can be interpreted as a decimal natural number if it is not empty and all the characters
-in it are digits.
-
-Use `Substring.isNat` to check whether the substring is such a substring.
--/
-def toNat? (s : Substring) : Option Nat :=
-  if s.isNat then
-    some <| s.foldl (fun n c => n*10 + (c.toNat - '0'.toNat)) 0
-  else
-    none
-
-/--
-Given a `Substring`, returns another one which has valid endpoints
-and represents the same substring according to `Substring.toString`.
-(Note, the substring may still be inverted, i.e. beginning greater than end.)
--/
-def repair : Substring → Substring
-  | ⟨s, b, e⟩ => ⟨s, if b.isValid s then b else s.rawEndPos, if e.isValid s then e else s.rawEndPos⟩
-
-/--
-Checks whether two substrings represent equal strings. Usually accessed via the `==` operator.
-
-Two substrings do not need to have the same underlying string or the same start and end positions;
-instead, they are equal if they contain the same sequence of characters.
--/
-def beq (ss1 ss2 : Substring) : Bool :=
-  let ss1 := ss1.repair
-  let ss2 := ss2.repair
-  ss1.bsize == ss2.bsize && String.Pos.Raw.substrEq ss1.str ss1.startPos ss2.str ss2.startPos ss1.bsize
-
-@[export lean_substring_beq]
-def Internal.beqImpl (ss1 ss2 : Substring) : Bool :=
-  Substring.beq ss1 ss2
-
-instance hasBeq : BEq Substring := ⟨beq⟩
-
-/--
-Checks whether two substrings have the same position and content.
-
-The two substrings do not need to have the same underlying string for this check to succeed.
--/
-def sameAs (ss1 ss2 : Substring) : Bool :=
-  ss1.startPos == ss2.startPos && ss1 == ss2
-
-/--
-Returns the longest common prefix of two substrings.
-
-The returned substring uses the same underlying string as `s`.
--/
-def commonPrefix (s t : Substring) : Substring :=
-  { s with stopPos := loop s.startPos t.startPos }
-where
-  /-- Returns the ending position of the common prefix, working up from `spos, tpos`. -/
-  loop spos tpos :=
-    if h : spos < s.stopPos ∧ tpos < t.stopPos then
-      if spos.get s.str == tpos.get t.str then
-        have := Nat.sub_lt_sub_left h.1 (String.Pos.Raw.lt_next s.str spos)
-        loop (spos.next s.str) (tpos.next t.str)
-      else
-        spos
-    else
-      spos
-  termination_by s.stopPos.byteIdx - spos.byteIdx
-
-/--
-Returns the longest common suffix of two substrings.
-
-The returned substring uses the same underlying string as `s`.
--/
-def commonSuffix (s t : Substring) : Substring :=
-  { s with startPos := loop s.stopPos t.stopPos }
-where
-  /-- Returns the starting position of the common prefix, working down from `spos, tpos`. -/
-  loop spos tpos :=
-    if h : s.startPos < spos ∧ t.startPos < tpos then
-      let spos' := spos.prev s.str
-      let tpos' := tpos.prev t.str
-      if spos'.get s.str == tpos'.get t.str then
-        have : spos' < spos := String.Pos.Raw.prev_lt_of_pos s.str spos (String.Pos.Raw.ne_zero_of_lt h.1)
-        loop spos' tpos'
-      else
-        spos
-    else
-      spos
-  termination_by spos.byteIdx
-
-/--
-If `pre` is a prefix of `s`, returns the remainder. Returns `none` otherwise.
-
-The substring `pre` is a prefix of `s` if there exists a `t : Substring` such that
-`s.toString = pre.toString ++ t.toString`. If so, the result is the substring of `s` without the
-prefix.
--/
-def dropPrefix? (s : Substring) (pre : Substring) : Option Substring :=
-  let t := s.commonPrefix pre
-  if t.bsize = pre.bsize then
-    some { s with startPos := t.stopPos }
-  else
-    none
-
-/--
-If `suff` is a suffix of `s`, returns the remainder. Returns `none` otherwise.
-
-The substring `suff` is a suffix of `s` if there exists a `t : Substring` such that
-`s.toString = t.toString ++ suff.toString`. If so, the result the substring of `s` without the
-suffix.
--/
-def dropSuffix? (s : Substring) (suff : Substring) : Option Substring :=
-  let t := s.commonSuffix suff
-  if t.bsize = suff.bsize then
-    some { s with stopPos := t.startPos }
-  else
-    none
-
-end Substring
 
 namespace String
 
-/--
-Removes the specified number of characters (Unicode code points) from the start of the string.
-
-If `n` is greater than `s.length`, returns `""`.
-
-Examples:
- * `"red green blue".drop 4 = "green blue"`
- * `"red green blue".drop 10 = "blue"`
- * `"red green blue".drop 50 = ""`
--/
-@[inline] def drop (s : String) (n : Nat) : String :=
-  (s.toSubstring.drop n).toString
-
-@[export lean_string_drop]
-def Internal.dropImpl (s : String) (n : Nat) : String :=
-  String.drop s n
-
-/--
-Removes the specified number of characters (Unicode code points) from the end of the string.
-
-If `n` is greater than `s.length`, returns `""`.
-
-Examples:
- * `"red green blue".dropRight 5 = "red green"`
- * `"red green blue".dropRight 11 = "red"`
- * `"red green blue".dropRight 50 = ""`
--/
-@[inline] def dropRight (s : String) (n : Nat) : String :=
-  (s.toSubstring.dropRight n).toString
-
-@[export lean_string_dropright]
-def Internal.dropRightImpl (s : String) (n : Nat) : String :=
-  String.dropRight s n
-
-/--
-Creates a new string that contains the first `n` characters (Unicode code points) of `s`.
-
-If `n` is greater than `s.length`, returns `s`.
-
-Examples:
-* `"red green blue".take 3 = "red"`
-* `"red green blue".take 1 = "r"`
-* `"red green blue".take 0 = ""`
-* `"red green blue".take 100 = "red green blue"`
--/
-@[inline] def take (s : String) (n : Nat) : String :=
-  (s.toSubstring.take n).toString
-
-/--
-Creates a new string that contains the last `n` characters (Unicode code points) of `s`.
-
-If `n` is greater than `s.length`, returns `s`.
-
-Examples:
-* `"red green blue".takeRight 4 = "blue"`
-* `"red green blue".takeRight 1 = "e"`
-* `"red green blue".takeRight 0 = ""`
-* `"red green blue".takeRight 100 = "red green blue"`
--/
-@[inline] def takeRight (s : String) (n : Nat) : String :=
-  (s.toSubstring.takeRight n).toString
-
-/--
-Creates a new string that contains the longest prefix of `s` in which `p` returns `true` for all
-characters.
-
-Examples:
-* `"red green blue".takeWhile (·.isLetter) = "red"`
-* `"red green blue".takeWhile (· == 'r') = "r"`
-* `"red green blue".takeWhile (· != 'n') = "red gree"`
-* `"red green blue".takeWhile (fun _ => true) = "red green blue"`
--/
-@[inline] def takeWhile (s : String) (p : Char → Bool) : String :=
-  (s.toSubstring.takeWhile p).toString
-
-/--
-Creates a new string by removing the longest prefix from `s` in which `p` returns `true` for all
-characters.
-
-Examples:
-* `"red green blue".dropWhile (·.isLetter) = " green blue"`
-* `"red green blue".dropWhile (· == 'r') = "ed green blue"`
-* `"red green blue".dropWhile (· != 'n') = "n blue"`
-* `"red green blue".dropWhile (fun _ => true) = ""`
--/
-@[inline] def dropWhile (s : String) (p : Char → Bool) : String :=
-  (s.toSubstring.dropWhile p).toString
-
-/--
-Creates a new string that contains the longest suffix of `s` in which `p` returns `true` for all
-characters.
-
-Examples:
-* `"red green blue".takeRightWhile (·.isLetter) = "blue"`
-* `"red green blue".takeRightWhile (· == 'e') = "e"`
-* `"red green blue".takeRightWhile (· != 'n') = " blue"`
-* `"red green blue".takeRightWhile (fun _ => true) = "red green blue"`
--/
-@[inline] def takeRightWhile (s : String) (p : Char → Bool) : String :=
-  (s.toSubstring.takeRightWhile p).toString
-
-/--
-Creates a new string by removing the longest suffix from `s` in which `p` returns `true` for all
-characters.
-
-Examples:
-* `"red green blue".dropRightWhile (·.isLetter) = "red green "`
-* `"red green blue".dropRightWhile (· == 'e') = "red green blu"`
-* `"red green blue".dropRightWhile (· != 'n') = "red green"`
-* `"red green blue".dropRightWhile (fun _ => true) = ""`
--/
-@[inline] def dropRightWhile (s : String) (p : Char → Bool) : String :=
-  (s.toSubstring.dropRightWhile p).toString
-
-/--
-Checks whether the first string (`s`) begins with the second (`pre`).
-
-`String.isPrefix` is a version that takes the potential prefix before the string.
-
-Examples:
- * `"red green blue".startsWith "red" = true`
- * `"red green blue".startsWith "green" = false`
- * `"red green blue".startsWith "" = true`
- * `"red".startsWith "red" = true`
--/
-@[inline] def startsWith (s pre : String) : Bool :=
-  s.toSubstring.take pre.length == pre.toSubstring
-
-/--
-Checks whether the first string (`s`) ends with the second (`post`).
-
-Examples:
- * `"red green blue".endsWith "blue" = true`
- * `"red green blue".endsWith "green" = false`
- * `"red green blue".endsWith "" = true`
- * `"red".endsWith "red" = true`
--/
-@[inline] def endsWith (s post : String) : Bool :=
-  s.toSubstring.takeRight post.length == post.toSubstring
-
-/--
-Removes trailing whitespace from a string.
-
-“Whitespace” is defined as characters for which `Char.isWhitespace` returns `true`.
-
-Examples:
-* `"abc".trimRight = "abc"`
-* `"   abc".trimRight = "   abc"`
-* `"abc \t  ".trimRight = "abc"`
-* `"  abc   ".trimRight = "  abc"`
-* `"abc\ndef\n".trimRight = "abc\ndef"`
--/
-@[inline] def trimRight (s : String) : String :=
-  s.toSubstring.trimRight.toString
-
-/--
-Removes leading whitespace from a string.
-
-“Whitespace” is defined as characters for which `Char.isWhitespace` returns `true`.
-
-Examples:
-* `"abc".trimLeft = "abc"`
-* `"   abc".trimLeft = "   abc"`
-* `"abc \t  ".trimLeft = "abc \t  "`
-* `"  abc   ".trimLeft = "abc   "`
-* `"abc\ndef\n".trimLeft = "abc\ndef\n"`
--/
-@[inline] def trimLeft (s : String) : String :=
-  s.toSubstring.trimLeft.toString
-
-/--
-Removes leading and trailing whitespace from a string.
-
-“Whitespace” is defined as characters for which `Char.isWhitespace` returns `true`.
-
-Examples:
-* `"abc".trim = "abc"`
-* `"   abc".trim = "abc"`
-* `"abc \t  ".trim = "abc"`
-* `"  abc   ".trim = "abc"`
-* `"abc\ndef\n".trim = "abc\ndef"`
--/
-@[inline] def trim (s : String) : String :=
-  s.toSubstring.trim.toString
-
-@[export lean_string_trim]
-def Internal.trimImpl (s : String) : String :=
-  String.trim s
-
-/--
-Repeatedly increments a position in a string, as if by `String.next`, while the predicate `p`
-returns `true` for the character at the position. Stops incrementing at the end of the string or
-when `p` returns `false` for the current character.
-
-Examples:
-* `let s := "   a  "; s.get (s.nextWhile Char.isWhitespace 0) = 'a'`
-* `let s := "a  "; s.get (s.nextWhile Char.isWhitespace 0) = 'a'`
-* `let s := "ba  "; s.get (s.nextWhile Char.isWhitespace 0) = 'b'`
--/
-@[inline] def Pos.Raw.nextWhile (s : String) (p : Char → Bool) (i : String.Pos.Raw) : String.Pos.Raw :=
-  Substring.takeWhileAux s s.rawEndPos p i
-
-@[deprecated Pos.Raw.nextWhile (since := "2025-10-10")]
-abbrev nextWhile (s : String) (p : Char → Bool) (i : String.Pos.Raw) : String.Pos.Raw :=
-  Pos.Raw.nextWhile s p i
-
-@[export lean_string_nextwhile]
-def Internal.nextWhileImpl (s : String) (p : Char → Bool) (i : String.Pos.Raw) : String.Pos.Raw :=
-  i.nextWhile s p
-
-/--
-Repeatedly increments a position in a string, as if by `String.next`, while the predicate `p`
-returns `false` for the character at the position. Stops incrementing at the end of the string or
-when `p` returns `true` for the current character.
-
-Examples:
-* `let s := "   a  "; s.get (s.nextUntil Char.isWhitespace 0) = ' '`
-* `let s := "   a  "; s.get (s.nextUntil Char.isLetter 0) = 'a'`
-* `let s := "a  "; s.get (s.nextUntil Char.isWhitespace 0) = ' '`
--/
-@[inline] def Pos.Raw.nextUntil (s : String) (p : Char → Bool) (i : String.Pos.Raw) : String.Pos.Raw :=
-  nextWhile s (fun c => !p c) i
-
-@[deprecated Pos.Raw.nextUntil (since := "2025-10-10")]
-def nextUntil (s : String) (p : Char → Bool) (i : String.Pos.Raw) : String.Pos.Raw :=
-  i.nextUntil s p
 
 /--
 Replaces each character in `s` with the result of applying `Char.toUpper` to it.
@@ -4455,70 +3297,6 @@ Examples:
 @[inline] def decapitalize (s : String) :=
   (0 : Pos.Raw).set s <| (0 : Pos.Raw).get s |>.toLower
 
-/--
-If `pre` is a prefix of `s`, returns the remainder. Returns `none` otherwise.
-
-The string `pre` is a prefix of `s` if there exists a `t : String` such that `s = pre ++ t`. If so,
-the result is `some t`.
-
-Use `String.stripPrefix` to return the string unchanged when `pre` is not a prefix.
-
-Examples:
- * `"red green blue".dropPrefix? "red " = some "green blue"`
- * `"red green blue".dropPrefix? "reed " = none`
- * `"red green blue".dropPrefix? "" = some "red green blue"`
--/
-def dropPrefix? (s : String) (pre : String) : Option Substring :=
-  s.toSubstring.dropPrefix? pre.toSubstring
-
-/--
-If `suff` is a suffix of `s`, returns the remainder. Returns `none` otherwise.
-
-The string `suff` is a suffix of `s` if there exists a `t : String` such that `s = t ++ suff`. If so,
-the result is `some t`.
-
-Use `String.stripSuffix` to return the string unchanged when `suff` is not a suffix.
-
-Examples:
- * `"red green blue".dropSuffix? " blue" = some "red green"`
- * `"red green blue".dropSuffix? " blu " = none`
- * `"red green blue".dropSuffix? "" = some "red green blue"`
--/
-def dropSuffix? (s : String) (suff : String) : Option Substring :=
-  s.toSubstring.dropSuffix? suff.toSubstring
-
-/--
-If `pre` is a prefix of `s`, returns the remainder. Returns `s` unmodified otherwise.
-
-The string `pre` is a prefix of `s` if there exists a `t : String` such that `s = pre ++ t`. If so,
-the result is `t`. Otherwise, it is `s`.
-
-Use `String.dropPrefix?` to return `none` when `pre` is not a prefix.
-
-Examples:
- * `"red green blue".stripPrefix "red " = "green blue"`
- * `"red green blue".stripPrefix "reed " = "red green blue"`
- * `"red green blue".stripPrefix "" = "red green blue"`
--/
-def stripPrefix (s : String) (pre : String) : String :=
-  s.dropPrefix? pre |>.map Substring.toString |>.getD s
-
-/--
-If `suff` is a suffix of `s`, returns the remainder. Returns `s` unmodified otherwise.
-
-The string `suff` is a suffix of `s` if there exists a `t : String` such that `s = t ++ suff`. If so,
-the result is `t`. Otherwise, it is `s`.
-
-Use `String.dropSuffix?` to return `none` when `suff` is not a suffix.
-
-Examples:
- * `"red green blue".stripSuffix " blue" = "red green"`
- * `"red green blue".stripSuffix " blu " = "red green blue"`
- * `"red green blue".stripSuffix "" = "red green blue"`
--/
-def stripSuffix (s : String) (suff : String) : String :=
-  s.dropSuffix? suff |>.map Substring.toString |>.getD s
-
 end String
 
 namespace String
@@ -4565,84 +3343,6 @@ theorem lt_iff {s t : String} : s < t ↔ s.data < t.data := .rfl
 
 namespace Pos.Raw
 
-theorem byteIdx_mk (n : Nat) : byteIdx ⟨n⟩ = n := rfl
-
-@[simp] theorem mk_zero : ⟨0⟩ = (0 : Pos.Raw) := rfl
-
-@[simp] theorem mk_byteIdx (p : Pos.Raw) : ⟨p.byteIdx⟩ = p := rfl
-
-@[deprecated byteIdx_offsetBy (since := "2025-10-08")]
-theorem add_byteIdx {p₁ p₂ : Pos.Raw} : (p₂.offsetBy p₁).byteIdx = p₁.byteIdx + p₂.byteIdx := by
-  simp
-
-@[deprecated byteIdx_offsetBy (since := "2025-10-08")]
-theorem add_eq {p₁ p₂ : Pos.Raw} : p₂.offsetBy p₁ = ⟨p₁.byteIdx + p₂.byteIdx⟩ := rfl
-
-@[deprecated byteIdx_unoffsetBy (since := "2025-10-08")]
-theorem sub_byteIdx (p₁ p₂ : Pos.Raw) : (p₁.unoffsetBy p₂).byteIdx = p₁.byteIdx - p₂.byteIdx := rfl
-
-@[deprecated byteIdx_add_char (since := "2025-10-10")]
-theorem addChar_byteIdx (p : Pos.Raw) (c : Char) : (p + c).byteIdx = p.byteIdx + c.utf8Size :=
-  byteIdx_add_char
-
-theorem add_char_eq (p : Pos.Raw) (c : Char) : p + c = ⟨p.byteIdx + c.utf8Size⟩ := rfl
-
-@[deprecated add_char_eq (since := "2025-10-10")]
-theorem addChar_eq (p : Pos.Raw) (c : Char) : p + c = ⟨p.byteIdx + c.utf8Size⟩ :=
-  add_char_eq p c
-
-theorem byteIdx_zero_add_char (c : Char) : ((0 : Pos.Raw) + c).byteIdx = c.utf8Size := by
-  simp only [byteIdx_add_char, byteIdx_zero, Nat.zero_add]
-
-@[deprecated byteIdx_zero_add_char (since := "2025-10-10")]
-theorem zero_addChar_byteIdx (c : Char) : ((0 : Pos.Raw) + c).byteIdx = c.utf8Size :=
-  byteIdx_zero_add_char c
-
-theorem zero_add_char_eq (c : Char) : (0 : Pos.Raw) + c = ⟨c.utf8Size⟩ := by rw [← byteIdx_zero_add_char]
-
-@[deprecated zero_add_char_eq (since := "2025-10-10")]
-theorem zero_addChar_eq (c : Char) : (0 : Pos.Raw) + c = ⟨c.utf8Size⟩ :=
-  zero_add_char_eq c
-
-theorem add_char_right_comm (p : Pos.Raw) (c₁ c₂ : Char) : p + c₁ + c₂ = p + c₂ + c₁ := by
-  simpa [Pos.Raw.ext_iff] using Nat.add_right_comm ..
-
-@[deprecated add_char_right_comm (since := "2025-10-10")]
-theorem addChar_right_comm (p : Pos.Raw) (c₁ c₂ : Char) : p + c₁ + c₂ = p + c₂ + c₁ :=
-  add_char_right_comm p c₁ c₂
-
-theorem ne_of_gt {i₁ i₂ : Pos.Raw} (h : i₁ < i₂) : i₂ ≠ i₁ := (ne_of_lt h).symm
-
-@[deprecated byteIdx_add_string (since := "2025-10-10")]
-theorem byteIdx_addString (p : Pos.Raw) (s : String) :
-    (p + s).byteIdx = p.byteIdx + s.utf8ByteSize := byteIdx_add_string
-
-@[deprecated byteIdx_addString (since := "2025-03-18")]
-abbrev addString_byteIdx := @byteIdx_add_string
-
-theorem addString_eq (p : Pos.Raw) (s : String) : p + s = ⟨p.byteIdx + s.utf8ByteSize⟩ := rfl
-
-theorem byteIdx_zero_add_string (s : String) : ((0 : Pos.Raw) + s).byteIdx = s.utf8ByteSize := by
-  simp only [byteIdx_add_string, byteIdx_zero, Nat.zero_add]
-
-@[deprecated byteIdx_zero_add_string (since := "2025-10-10")]
-theorem byteIdx_zero_addString (s : String) : ((0 : Pos.Raw) + s).byteIdx = s.utf8ByteSize :=
-  byteIdx_zero_add_string s
-
-@[deprecated byteIdx_zero_addString (since := "2025-03-18")]
-abbrev zero_addString_byteIdx := @byteIdx_zero_add_string
-
-theorem zero_add_string_eq (s : String) : (0 : Pos.Raw) + s = ⟨s.utf8ByteSize⟩ := by
-  rw [← byteIdx_zero_add_string]
-
-@[deprecated zero_add_string_eq (since := "2025-10-10")]
-theorem zero_addString_eq (s : String) : (0 : Pos.Raw) + s = ⟨s.utf8ByteSize⟩ :=
-  zero_add_string_eq s
-
-@[simp] theorem mk_le_mk {i₁ i₂ : Nat} : Pos.Raw.mk i₁ ≤ Pos.Raw.mk i₂ ↔ i₁ ≤ i₂ := .rfl
-
-@[simp] theorem mk_lt_mk {i₁ i₂ : Nat} : Pos.Raw.mk i₁ < Pos.Raw.mk i₂ ↔ i₁ < i₂ := .rfl
-
 @[simp] theorem get!_eq_get (s : String) (p : Pos.Raw) : p.get! s = p.get s := rfl
 
 @[simp] theorem get'_eq (s : String) (p : Pos.Raw) (h) : get' s p h = get s p := rfl
@@ -4688,13 +3388,3 @@ theorem toString_eq_singleton {c : Char} : c.toString = String.singleton c := rf
 end Char
 
 open String
-
-namespace Substring
-
-@[simp] theorem prev_zero (s : Substring) : s.prev 0 = 0 := by simp [prev]
-
-@[simp] theorem prevn_zero (s : Substring) : ∀ n, s.prevn n 0 = 0
-  | 0 => rfl
-  | n+1 => by simp [prevn, prevn_zero s n]
-
-end Substring
