src/lake/Lake/Toml/Data/Value.lean
@@ -10,7 +10,7 @@ public import Init.Data.Float
 public import Lake.Toml.Data.Dict
 public import Lake.Toml.Data.DateTime
 import Lake.Util.String
-import Init.Data.String.Basic
+import Init.Data.String.TakeDrop
 
 /-!
 # TOML Value
